stated refinement soundness, removed old code

FiatFormal/Language/Refinement.v
@@ -41,9 +41,7 @@ Definition getCod (m : method) :=
 Definition getBody (m : method) :=
   m.(body).
 
-(* Definition wfRefinement (aOld aNew : adt) :=. *)
-
-Inductive refinesADT'
+Inductive refinesADT
            (ProofBuilder : propcon -> list exp -> Prop)
            (ds : defs)
            (ProofBuilderOK : forall ke te pc xs ts,
@@ -68,160 +66,16 @@ Inductive refinesADT'
                 (XNApp (bodyOld) (repsOld >< vs))
                 (XTup ((nil :> v) :> repOld'))
           /\ R repOld' repNew'))
-          -> refinesADT' ProofBuilder ds ProofBuilderOK
+          -> refinesADT ProofBuilder ds ProofBuilderOK
                         (IADT repOld methodsOld sigsOld)
                         (IADT repNew methodsNew sigsNew).
 
-(* Definition refinesADT *)
-(*            (ProofBuilder : propcon -> list exp -> Prop) *)
-(*            (ds : defs) *)
-(*            (ProofBuilderOK : forall ke te pc xs ts, *)
-(*                ProofBuilder pc xs *)
-(*                -> getPropDef pc ds = Some (DefProp pc ts) *)
-(*                -> Forall2 (TYPE ds ke te) xs ts) *)
-(*            (aOld aNew : adt) := *)
-
-
-(*   forall repTypeOld repTypeNew, *)
-(*     getRepType aOld = repTypeOld *)
-(*     -> getRepType aNew = repTypeNew *)
-(*     -> exists (absRel : exp -> exp -> Prop), (* This is not correct? *) *)
-(*       forall n mOld mNew *)
-(*         methodsNew methodsOld *)
-(*         mDomNew mDomOld *)
-(*         arityNew arityOld *)
-(*         repsNew repsOld *)
-(*         bodyNew bodyOld *)
-(*         vs, *)
-
-(*         getMethods aNew = methodsNew *)
-(*         -> getMethods aOld = methodsOld *)
-(*         -> length methodsNew = length methodsOld *)
-(*         -> get n methodsNew = Some mNew *)
-(*         -> get n methodsOld = Some mOld *)
-(*         -> getDom mNew = mDomNew *)
-(*         -> getDom mOld = mDomOld *)
-(*         -> mDomNew = mDomOld *)
-(*         -> getArity mOld = arityOld *)
-(*         -> getArity mNew = arityNew *)
-(*         -> arityNew = arityOld *)
-(*         -> getBody mNew = bodyNew *)
-(*         -> getBody mOld = bodyOld *)
-
-(*         -> length vs = length mDomNew *)
-(*         -> Forall wnfX vs *)
-(*         -> length repsNew = arityNew *)
-(*         -> Forall2 (absRel) repsOld repsNew *)
-
-(*         -> forall v repNew', *)
-(*             STEPS ProofBuilder ds ProofBuilderOK *)
-(*                   (XNApp (bodyNew) (repsNew >< vs)) *)
-(*                   (XTup ((nil :> v) :> repNew')) *)
-(*             -> exists repOld', *)
-(*               STEPS ProofBuilder ds ProofBuilderOK *)
-(*                     (XNApp (bodyOld) (repsOld >< vs)) *)
-(*                     (XTup ((nil :> v) :> repOld')) *)
-(*               /\ absRel repOld' repNew'. *)
-
-(* Definition getArity (ts : list ty) (x : exp) (m : (XNFun ts x)) := *)
-(*   length ts. *)
-
-(* Definition getFuns := term. *)
-
-(* Definition getOps (a : adt) : list (option exp) := *)
-(*   match a with *)
-(*   | IADT r x s => match x with *)
-(*                  | XTup xs => match xs with *)
-(*                                | ((XNFun ts x) as f) :: xs' => Some f :: (getOps a *)
-(*                                | _ :: xs' => *)
-(*                                | nil => nil *)
-(*                                end *)
-(*                  | _ => nil *)
-(*                                                                          end. *)
-
-(* Definition getMethods (a : adt) : list method := *)
-(* match a with *)
-(* | IADT r ms ts => ms *)
-(* end. *)
-
-(* Definition getArity (m : method) := *)
-(* match m with. *)
-
-(* Definition refinesADT (aOld aNew : adt) := *)
-(*   getBody aOld = (XTup ms) *)
-(*   -> Forall2 (fun m => exists ts x, m = (XNFun ts x)) ms *)
-(*   exists (absRel : getRepType aOld -> getRepType aNew -> Prop), *)
-(*     -> length ms = n *)
-(*     -> *)
-
-(*   forall methodsOld methodsNew methodOld methodNew i numMethods, *)
-(*     getMethods aOld = methodsOld *)
-(*     -> getMethods aNew = methodsNew *)
-(*     -> length methodsOld = length methodsNew *)
-(*     -> get i methodsNew = methodNew *)
-(*     -> get i methodsOld = methodOld *)
-(*     -> forall (reps_o : list (getRepType aOld)) (reps_n : list (getRepType aNew)) *)
-(*         (arity : nat) (domSize : nat) xs vPairNew vRes vPairOld rep_n', *)
-(*         arity = getArity methodNew *)
-(*         -> length reps_o = arity *)
-(*         -> length reps_n = arity *)
-(*         -> length xs = domSize *)
-(*         -> Forall2 (absRel) reps_o reps_n *)
-(*         -> STEPS (XNApp opNew (reps_n >< xs)) vPairNew *)
-(*         -> XProj 0 vPairNew = rep_n' *)
-(*         -> XProj 1 vPairNew = vRes *)
-(*         -> exists rep_o', *)
-(*             (STEPS (XNApp opOld (reps_o >< xs)) vPairOld *)
-(*             /\ XProj 0 vPairOld = rep_o' *)
-(*             /\ XProj 1 vPairOld = vRes) *)
-(*             /\ absRel rep_o' rep_n'. *)
-
-(* Definition ADTrefines (aOld aNew : adt) := *)
-(*   wfADT aOld -> wfADT aNew -> *)
-(*   exists (absRel : getRepType aOld -> getRepType aNew -> Prop), *)
-(*   forall methodsOld methodsNew methodOld methodNew i numMethods, *)
-(*     getMethods aOld = methodsOld *)
-(*     -> getMethods aNew = methodsNew *)
-(*     -> length methodsOld = length methodsNew *)
-(*     -> get i methodsNew = methodNew *)
-(*     -> get i methodsOld = methodOld *)
-(*     -> forall (reps_o : list (getRepType aOld)) (reps_n : list (getRepType aNew)) *)
-(*         (arity : nat) (domSize : nat) xs vPairNew vRes vPairOld rep_n', *)
-(*         arity = getArity methodNew *)
-(*         -> length reps_o = arity *)
-(*         -> length reps_n = arity *)
-(*         -> length xs = domSize *)
-(*         -> Forall2 (absRel) reps_o reps_n *)
-(*         -> STEPS (XNApp opNew (reps_n >< xs)) vPairNew *)
-(*         -> XProj 0 vPairNew = rep_n' *)
-(*         -> XProj 1 vPairNew = vRes *)
-(*         -> exists rep_o', *)
-(*             (STEPS (XNApp opOld (reps_o >< xs)) vPairOld *)
-(*             /\ XProj 0 vPairOld = rep_o' *)
-(*             /\ XProj 1 vPairOld = vRes) *)
-(*             /\ absRel rep_o' rep_n'. *)
-
-
-(* Definition ADTrefines' (aOld aNew : adt) := *)
-(*   exists (absRel : getRepType aOld -> getRepType aNew -> Prop), *)
-(*   forall opsOld opsNew opOld opNew i numMethods, *)
-(*     getOps aOld = opsOld *)
-(*     -> getOps aNew = opsNew *)
-(*     -> length opsOld = length opsNew *)
-(*     -> get i opsNew = opNew *)
-(*     -> get i opsOld = opOld *)
-(*     -> forall (reps_o : list (getRepType aOld)) (reps_n : list (getRepType aNew)) *)
-(*         (arity : nat) (domSize : nat) xs vPairNew vRes vPairOld rep_n', *)
-(*         arity = getArity opNew *)
-(*         -> length reps_o = arity *)
-(*         -> length reps_n = arity *)
-(*         -> length xs = domSize *)
-(*         -> Forall2 (absRel) reps_o reps_n *)
-(*         -> STEPS (XNApp opNew (reps_n >< xs)) vPairNew *)
-(*         -> XProj 0 vPairNew = rep_n' *)
-(*         -> XProj 1 vPairNew = vRes *)
-(*         -> exists rep_o', *)
-(*             (STEPS (XNApp opOld (reps_o >< xs)) vPairOld *)
-(*             /\ XProj 0 vPairOld = rep_o' *)
-(*             /\ XProj 1 vPairOld = vRes) *)
-(*             /\ absRel rep_o' rep_n'. *)
+Theorem refinementSoundess : forall pb ds pbOK ao an p,
+    refinesADT pb ds pbOK ao an ->
+    refinesP (PLET ao p) (PLET an p).
+Proof.
+  unfold refinesP.
+  intros.
+  inverts H.
+  dest H1.
+Admitted.
